compiler/src/FlatToRiscv32Specifics.v
@@ -5,13 +5,13 @@ Require Import compiler.FlatToRiscvBitWidthSpecifics.
 Require Import riscv.Memory.
 
 
-Instance FlatToRiscv32Specifics(mem: Set)
-         {MW: MachineWidth (word 32)}{IsMem: Memory mem (word 32)}
-  : FlatToRiscvBitWidthSpecifics (word 32) mem := {|
+Instance FlatToRiscv32Specifics{MW: MachineWidth (word 32)}{MF: MemoryFunctions (word 32)}
+  : FlatToRiscvBitWidthSpecifics (word 32)  := {|
 
   BitWidth := BW32;
 
   loadWordwXLEN := loadWord;
-  
+
   storeWordwXLEN := storeWord;
+
 |}.
